Give maps a proper abstraction relation

src/goose_lang/map_triples.v
@@ -109,37 +109,42 @@ Proof.
     eexists _, _, _, _; intuition eauto.
 Qed.
 
-Definition wp_NewMap stk E T :
+Definition is_map (mref:loc) (m: gmap u64 val * val): iProp Σ :=
+  ∃ mv, ⌜map_val mv = Some m⌝ ∗ mref ↦ Free mv.
+
+Definition wp_NewMap stk E t :
   {{{ True }}}
-    NewMap T @ stk; E
-  {{{ mref mv def, RET #mref;
-    mref ↦ Free mv ∗ ⌜map_val mv = Some (∅, def)⌝ }}}.
+    NewMap t @ stk; E
+  {{{ mref, RET #mref;
+      is_map mref (∅, zero_val t) }}}.
 Proof.
   iIntros (Φ) "_ HΦ".
   wp_apply wp_alloc_zero.
   iIntros (mref) "Hm".
   iApply "HΦ".
 
-  (* This seems messy.. *)
   rewrite /struct_mapsto /= loc_add_0.
   iDestruct "Hm" as "[[Hm _] %]".
-  iFrame.
-  auto.
+  iExists _; iSplitR; auto.
+  by rewrite /=.
 Qed.
 
-Definition wp_MapGet stk E mref (m: gmap u64 val * val) mv k :
-  {{{ mref ↦ Free mv ∗ ⌜map_val mv = Some m⌝ }}}
+Definition wp_MapGet stk E mref (m: gmap u64 val * val) k :
+  {{{ is_map mref m }}}
     MapGet #mref #k @ stk; E
   {{{ v ok, RET (v, #ok); ⌜map_get m k = (v, ok)⌝ ∗
-                          mref ↦ Free mv }}}.
+                          is_map mref m }}}.
 Proof.
-  iIntros (Φ) "[Hmref %] HΦ".
+  iIntros (Φ) "Hmref HΦ".
+  iDestruct "Hmref" as (mv H) "Hmref".
   wp_call.
   wp_load.
   wp_pure (_ _).
   iAssert (∀ v ok, ⌜map_get m k = (v, ok)⌝ -∗ Φ (v, #ok)%V)%I with "[Hmref HΦ]" as "HΦ".
   { iIntros (v ok) "%".
-    by iApply ("HΦ" with "[$Hmref]"). }
+    iApply ("HΦ" with "[Hmref]").
+    iSplitR; auto.
+    iExists mv; by iFrame. }
   iLöb as "IH" forall (m mv H).
   wp_call.
   destruct (map_val_split _ _ H).
@@ -162,30 +167,31 @@ Proof.
         destruct m'; eauto.
 Qed.
 
-Definition wp_MapInsert stk E mref (m: gmap u64 val * val) mv k v' :
-  {{{ mref ↦ Free mv ∗ ⌜map_val mv = Some m⌝ }}}
+Definition wp_MapInsert stk E mref (m: gmap u64 val * val) k v' :
+  {{{ is_map mref m }}}
     MapInsert #mref #k v' @ stk; E
-  {{{ mv', RET #(); mref ↦ Free mv' ∗
-                    ⌜map_val mv' = Some (map_insert m k v')⌝ }}}.
+  {{{ RET #(); is_map mref (map_insert m k v') }}}.
 Proof.
-  iIntros (Φ) "[Hmref %] HΦ".
+  iIntros (Φ) "Hmref HΦ".
+  iDestruct "Hmref" as (mv ?) "Hmref".
   wp_call.
   wp_load.
   wp_store.
-  iApply ("HΦ" with "[$Hmref]").
+  iApply ("HΦ" with "[Hmref]").
+  iExists _; iFrame.
   iPureIntro.
   simpl.
   rewrite H.
   destruct m; simpl; auto.
 Qed.
 
-Definition wp_MapDelete stk E mref (m: gmap u64 val * val) mv k :
-  {{{ mref ↦ Free mv ∗ ⌜map_val mv = Some m⌝ }}}
+Definition wp_MapDelete stk E mref (m: gmap u64 val * val) k :
+  {{{ is_map mref m }}}
     MapDelete #mref #k @ stk; E
-  {{{ mv', RET #(); mref ↦ Free mv' ∗
-                    ⌜map_val mv' = Some (map_del m k)⌝ }}}.
+  {{{ RET #(); is_map mref (map_del m k) }}}.
 Proof.
-  iIntros (Φ) "[Hmref %] HΦ".
+  iIntros (Φ) "Hmref HΦ".
+  iDestruct "Hmref" as (mv ?) "Hmref".
   wp_call.
   wp_load.
   wp_pure (Rec _ _ _).
